LogRel/STLC/OpenClose.lean
@@ -19,5 +19,13 @@ def closedb_at (e : Expr) (i : ℕ) : Prop :=
   | .unit => true
 
 @[simp]
+def subst (x : ℕ) (v : Expr) : Expr -> Expr
+  | .bvar i => .bvar i
+  | .fvar y => if x = y then v else .fvar y
+  | .lam e => .lam (subst x v e)
+  | .app f arg => .app (subst x v f) (subst x v arg)
+  | .unit => .unit
+
+@[simp]
 def lc e :=
   closedb_at e 0
